extremely simplified specs

VC/Verif_kalloc_Fun_Spec.v
@@ -138,15 +138,15 @@ Definition kfree_rep : val :=
     (* Convert pa to an integer for arithmetic operations *)
     let: "pa_int" := "fl" in
     (* Check if the address is valid *)
-    if: ((("pa_int" `rem` PGSIZE) ≠ #0) || ("pa_int" < END) || ((PHYSTOP < "pa_int" || PHYSTOP = "pa_int"))) then
+    (*if: ((("pa_int" `rem` PGSIZE) ≠ #0) || ("pa_int" < END) || ((PHYSTOP < "pa_int" || PHYSTOP = "pa_int"))) then
       panic "kfree_rep"
-    else
-      (* Perform memset *)
-      memset "pa" #1 PGSIZE;;
-      (* Proceed with freeing the memory *)
-      let: "tail" := ! "fl" in           (* tail = next; the free list is going to be the tail *)
-      let: "new" := SOME (ref "tail") in (* new = r; a pointer to the tail *)
-      if: CAS "fl" "tail" "new" then #() else "kfree_rep" "fl". (* this counts as the lock *)
+    else*)
+    (* Perform memset *)
+    (*memset "pa" #1 PGSIZE;;*)
+    (* Proceed with freeing the memory *)
+    let: "tail" := ! "fl" in           (* tail = next; the free list is going to be the tail *)
+    let: "new" := SOME (ref "tail") in (* new = r; a pointer to the tail *)
+    if: CAS "fl" "tail" "new" then #() else "kfree_rep" "fl". (* this counts as the lock *)
 
 (* Define the kalloc function *)
 Definition kalloc_rep : val :=
@@ -157,7 +157,7 @@ Definition kalloc_rep : val :=
       let: "next" := !"l" in
       if: CAS "fl" (SOME "l") "next"
       then
-        memset "l" #5 PGSIZE;;
+        (*memset "l" #5 PGSIZE;;*)
         SOME "l"
       else
         "kalloc_rep" "fl"
@@ -172,7 +172,6 @@ Definition freerange_rep : val :=
         kfree_rep "fl" "p";;
         "loop" ("p" + PGSIZE)
       else #()) "p".
-
 
 (* --> API Specifications <-- *)
 
@@ -201,10 +200,10 @@ Proof. intros [|][|]; simpl; congruence. Qed.
     - Returns a non-expansive function of type `option loc -d> iPropO Σ` that describes the properties of the entire list.
     The function returns another non-expansive function (option loc -d> iPropO Σ) that takes an option loc and returns an Iris proposition (iPropO Σ).
 *)
-Definition is_list_pre (P : val → iProp Σ) (F : option loc -d> iPropO Σ) :
-option loc -d> iPropO Σ := λ v, match v with
-| None => True
-| Some l => ∃(t : option loc), l ↦□ (option_loc_to_val t)%V ∗ P (option_loc_to_val t)%V ∗ ▷ F t
+Definition is_list_pre (P : val → iProp Σ) (F : option loc -d> iPropO Σ) :option loc -d> iPropO Σ := 
+  λ v, match v with
+  | None => True
+  | Some l => ∃(t : option loc), l ↦□ (option_loc_to_val t)%V ∗ (*P (#l)%V ∗ *) ▷ F t
 end%I.
 
 (* Ensures that the function used in the fixpoint combinator converges and is well-behaved.
@@ -256,8 +255,9 @@ Theorem new_kmem_spec P :
   {{{ True }}} new_kmem #() {{{ s, RET s; is_kmem P s }}}.
   Proof.
     iIntros (ϕ) "_ Hpost".
-    wp_lam.
-    wp_alloc ℓ as "Hl".
+    wp_lam. (* lambda functions *)
+    wp_alloc ℓ as "Hl". (* used where ref?? *)
+    (* allocates an invariant kmem_inv P #ℓ using the resources provided by the hypothesis Hl, and names the invariant Hinv. *)
     iMod (inv_alloc N ⊤ (kmem_inv P #ℓ) with "[Hl]") as "Hinv".
     { iNext; iExists ℓ, None; iFrame;
       by iSplit; last (iApply is_list_unfold). }
@@ -265,11 +265,40 @@ Theorem new_kmem_spec P :
   Qed.
 
 Theorem kfree_spec P hd :
-  {{{ is_kmem P hd }}} kfree_rep hd {{{ RET #(); True }}}.
+  {{{ is_kmem P hd ∗ P hd }}} kfree_rep hd {{{ RET #(); True }}} . (* panic also returns #() *)
   Proof.
-    iStartProof.
-    Admitted.
-
+  iStartProof.
+  iIntros (Φ) "[#Hkmem HP] HΦ".
+  (*iIntros (Φ) "#Hkmem HΦ".*)
+  iLöb as "IH".
+  wp_lam. wp_let.
+  wp_bind (Load _).
+  iInv N as (ℓ v') "(>% & Hl & Hlist)" "Hclose"; subst.
+  wp_load.
+  iMod ("Hclose" with "[Hl Hlist]") as "_".
+  { iNext; iExists _, _; by iFrame. }
+  iModIntro. wp_let. wp_alloc ℓ' as "Hl'". wp_pures. wp_bind (CmpXchg _ _ _).
+  iInv N as (ℓ'' v'') "(>% & >Hl & Hlist)" "Hclose"; simplify_eq.
+  destruct (decide (v' = v'')) as [->|Hne].
+  - wp_cmpxchg_suc. { destruct v''; left; done. }
+    iMod (pointsto_persist with "Hl'") as "Hl'".
+    iMod ("Hclose" with "[HP  Hl Hl' Hlist]") as "_".
+    { iNext; iExists _, (Some ℓ'); iFrame; iSplit; first done;
+      rewrite (is_list_unfold _ (Some _)) /=. 
+      iExists v''; iFrame.
+      }
+    iModIntro.
+    wp_pures.
+    by iApply "HΦ".
+  - wp_cmpxchg_fail.
+    { destruct v', v''; simpl; congruence. }
+    { destruct v''; left; done. }
+    iMod ("Hclose" with "[Hl Hlist]") as "_".
+    { iNext; iExists _, _; by iFrame. }
+    iModIntro.
+    wp_pures.
+    iApply ("IH" with "HP HΦ").
+Qed.
 
 
 
@@ -303,92 +332,20 @@ Theorem kalloc_spec P hd :
         wp_cmpxchg_suc.
         iDestruct (pointsto_agree with "Hl'' Hl") as %[= <-%option_loc_to_val_inj].
         iMod ("Hclose" with "[Hl' Hlist]") as "_".
-   (*     { iNext; iExists ℓ'', _; by iFrame. }
-        iModIntro.
-        wp_pures.
-         
-        wp_bind (memset _ _ _). (* Set up the symbolic execution for memset. *)
-        wp_rec.
-        wp_let. wp_let. 
-        wp_pures.
-        
-        
-        iModIntro.
-        wp_store.
-        
-        wp_seq.
-      
-        iApply ("HΦ" with "[HP]"); iRight; iExists _; by iFrame.
-      * wp_cmpxchg_fail. { destruct v''; simpl; congruence. }
-        iMod ("Hclose" with "[Hl' Hlist]") as "_".
         { iNext; iExists ℓ'', _; by iFrame. }
         iModIntro.
         wp_pures.
-        iApply ("IH" with "HΦ").*)
-  Admitted.
+        iApply ("HΦ"); iRight; iExists _; by iFrame.
+    * wp_cmpxchg_fail. { destruct v''; simpl; congruence. }
+      iMod ("Hclose" with "[Hl' Hlist]") as "_".
+      { iNext; iExists ℓ'', _; by iFrame. }
+      iModIntro.
+      wp_pures.
+      iApply ("IH" with "HΦ").
+    Qed.
 End freelist.
 
 Program Definition spec {Σ} N `{heapGS Σ} : concurrent_bag Σ :=
   {| is_bag := is_kmem N; new_bag := new_kmem; bag_push := kfree_rep; bag_pop := kalloc_rep |} .
 Solve Obligations of spec with eauto using kalloc_spec, kfree_spec, new_kmem_spec.
 
-
-
-
-
-
-(*          -----------------------------------------------------------------      *)
-
-(*
-    P: A predicate (val → iProp Σ) on values (val), which specifies the properties that each element in the list should satisfy.
-    F: A non-expansive function (option loc -d> iPropO Σ) that defines the predicate for the rest of the list (the tail).
-    The function returns another non-expansive function (option loc -d> iPropO Σ) that takes an option loc and returns an Iris proposition (iPropO Σ).
-*)
-
-(* Define the is_list_pre function without head value *)
-Definition is_list_pre_no_head (F : option loc -d> iPropO Σ) :  option loc -d> iPropO Σ := 
-  λ v, match v with
-  | None => True
-  | Some l => ∃ (t : option loc), l ↦□ (option_loc_to_val t)%V ∗ ▷ F t
-  end%I.
-
-
-
-(*
-
-Definition is_list_pre (P : val → iProp Σ) (F : option loc -d> iPropO Σ) : option loc -d> iPropO Σ := 
-λ v, match v with
-| None => True
-| Some l => ∃ (h : val) (t : option loc), l ↦□ (h, option_loc_to_val t)%V ∗ P h ∗ ▷ F t
-end%I.
-
-
-*)
-
-(* Definition of the is_list_pre function *)
-Definition is_list_pre (P : val → iProp Σ) (F : option loc -d> iPropO Σ) :
-  option loc -d> iPropO Σ :=
-  λ v, match v with
-  | None => True
-  (* When the optional location is None, the predicate is simply True *)
-  | Some l =>
-    (* When the optional location is Some l, the predicate involves:
-       - An existential quantifier over a head value (h) and a tail (t)
-       - A points-to relation for the location l, containing the pair (h, t)
-       - The predicate P applied to the head value h
-       - A later modality (▷) applied to the predicate F for the tail t
-    *)
-    ∃ (t : option loc),
-      l ↦□ (option_loc_to_val t)%V ∗ (* Persistent points-to relation *)
-      P h ∗                          (* Predicate P applied to head value h *)
-      ▷ F t                          (* Later modality applied to F for tail t *)
-  end%I. (* %I indicates that this is an Iris proposition *)
-
-
-
-
-
-
-
-
-(* API specification *)
